<?xml version="1.0" encoding="UTF-8"?>
<!DOCTYPE rdf:RDF [
	<!ENTITY cmns-av "https://www.omg.org/spec/Commons/AnnotationVocabulary/">
	<!ENTITY cmns-cls "https://www.omg.org/spec/Commons/Classifiers/">
	<!ENTITY cmns-col "https://www.omg.org/spec/Commons/Collections/">
	<!ENTITY cmns-dsg "https://www.omg.org/spec/Commons/Designators/">
	<!ENTITY cmns-id "https://www.omg.org/spec/Commons/Identifiers/">
	<!ENTITY cmns-qtu "https://www.omg.org/spec/Commons/QuantitiesAndUnits/">
	<!ENTITY cmns-txt "https://www.omg.org/spec/Commons/TextDatatype/">
	<!ENTITY dct "http://purl.org/dc/terms/">
	<!ENTITY idmp-chg "https://spec.pistoiaalliance.org/idmp/ontology/META/ChangeManagement/">
	<!ENTITY idmp-dtp "https://spec.pistoiaalliance.org/idmp/ontology/ISO/ISO21090-HarmonizedDatatypes/">
	<!ENTITY idmp-ucum "https://spec.pistoiaalliance.org/idmp/ontology/EXT/Extensions/UnifiedCodeForUnitsOfMeasure/">
	<!ENTITY idmp-uom "https://spec.pistoiaalliance.org/idmp/ontology/ISO/ISO11240-UnitsOfMeasurement/">
	<!ENTITY owl "http://www.w3.org/2002/07/owl#">
	<!ENTITY rdf "http://www.w3.org/1999/02/22-rdf-syntax-ns#">
	<!ENTITY rdfs "http://www.w3.org/2000/01/rdf-schema#">
	<!ENTITY skos "http://www.w3.org/2004/02/skos/core#">
	<!ENTITY xsd "http://www.w3.org/2001/XMLSchema#">
]>
<rdf:RDF xml:base="https://spec.pistoiaalliance.org/idmp/ontology/EXT/Extensions/UnifiedCodeForUnitsOfMeasure/"
	xmlns:cmns-av="https://www.omg.org/spec/Commons/AnnotationVocabulary/"
	xmlns:cmns-cls="https://www.omg.org/spec/Commons/Classifiers/"
	xmlns:cmns-col="https://www.omg.org/spec/Commons/Collections/"
	xmlns:cmns-dsg="https://www.omg.org/spec/Commons/Designators/"
	xmlns:cmns-id="https://www.omg.org/spec/Commons/Identifiers/"
	xmlns:cmns-qtu="https://www.omg.org/spec/Commons/QuantitiesAndUnits/"
	xmlns:cmns-txt="https://www.omg.org/spec/Commons/TextDatatype/"
	xmlns:dct="http://purl.org/dc/terms/"
	xmlns:idmp-chg="https://spec.pistoiaalliance.org/idmp/ontology/META/ChangeManagement/"
	xmlns:idmp-dtp="https://spec.pistoiaalliance.org/idmp/ontology/ISO/ISO21090-HarmonizedDatatypes/"
	xmlns:idmp-ucum="https://spec.pistoiaalliance.org/idmp/ontology/EXT/Extensions/UnifiedCodeForUnitsOfMeasure/"
	xmlns:idmp-uom="https://spec.pistoiaalliance.org/idmp/ontology/ISO/ISO11240-UnitsOfMeasurement/"
	xmlns:owl="http://www.w3.org/2002/07/owl#"
	xmlns:rdf="http://www.w3.org/1999/02/22-rdf-syntax-ns#"
	xmlns:rdfs="http://www.w3.org/2000/01/rdf-schema#"
	xmlns:skos="http://www.w3.org/2004/02/skos/core#"
	xmlns:xsd="http://www.w3.org/2001/XMLSchema#">
	
	<owl:Ontology rdf:about="https://spec.pistoiaalliance.org/idmp/ontology/EXT/Extensions/UnifiedCodeForUnitsOfMeasure/">
		<rdfs:label>Unified Code for Units of Measure (UCUM) Ontology</rdfs:label>
		<dct:abstract>The Unified Code for Units of Measure (UCUM) was developed by Regenstrief Institute and the UCUM Organization as a unambiguous system of units and their combinations. This ontology specifies the UCUM code system, and is intended to cover the units of measure specified therein, as described by the ISO 11240:2012 Health informatics - Identification of medicinal products - Data elements and structures for the unique identification and exchange of units of measurement standard.</dct:abstract>
		<dct:license rdf:datatype="&xsd;anyURI">http://opensource.org/licenses/MIT</dct:license>
		<owl:imports rdf:resource="https://spec.pistoiaalliance.org/idmp/ontology/ISO/ISO11240-UnitsOfMeasurement/"/>
		<owl:imports rdf:resource="https://spec.pistoiaalliance.org/idmp/ontology/ISO/ISO21090-HarmonizedDatatypes/"/>
		<owl:imports rdf:resource="https://spec.pistoiaalliance.org/idmp/ontology/META/ChangeManagement/"/>
		<owl:imports rdf:resource="https://www.omg.org/spec/Commons/AnnotationVocabulary/"/>
		<owl:imports rdf:resource="https://www.omg.org/spec/Commons/Classifiers/"/>
		<owl:imports rdf:resource="https://www.omg.org/spec/Commons/Collections/"/>
		<owl:imports rdf:resource="https://www.omg.org/spec/Commons/Designators/"/>
		<owl:imports rdf:resource="https://www.omg.org/spec/Commons/Identifiers/"/>
		<owl:imports rdf:resource="https://www.omg.org/spec/Commons/QuantitiesAndUnits/"/>
		<owl:imports rdf:resource="https://www.omg.org/spec/Commons/TextDatatype/"/>
		<owl:versionIRI rdf:resource="https://spec.pistoiaalliance.org/idmp/ontology/EXT/20220901/Extensions/UnifiedCodeForUnitsOfMeasure/"/>
		<idmp-chg:hasMaturityLevel rdf:resource="&idmp-chg;Informative"/>
		<cmns-av:copyright>Copyright (c) 2022 EDM Council, Inc.</cmns-av:copyright>
		<cmns-av:copyright>Copyright (c) 2022 Pistoia Alliance, Inc.</cmns-av:copyright>
	</owl:Ontology>
	
	<owl:NamedIndividual rdf:about="&idmp-ucum;AmountOfSubstance">
		<rdf:type rdf:resource="&cmns-qtu;BaseQuantityKind"/>
		<rdfs:label>amount of substance</rdfs:label>
		<dct:source>https://ucum.org/ucum.html#section-Base-Units</dct:source>
		<skos:definition>base quantity kind defined in the Unified Code for Units Of Measure (UCUM) System of Units for the quantity or number of discrete atomic-scale particles in a given sample of matter divided by the Avogadro constant</skos:definition>
		<cmns-av:explanatoryNote>The particles or entities may be molecules, atoms, ions, electrons, or other, depending on the context, and should be specified.</cmns-av:explanatoryNote>
		<cmns-av:symbol>n</cmns-av:symbol>
		<cmns-dsg:isDefinedIn rdf:resource="&idmp-ucum;UnifiedCodeForUnitsOfMeasure"/>
	</owl:NamedIndividual>
	
	<owl:NamedIndividual rdf:about="&idmp-ucum;Ampoule">
		<rdf:type rdf:resource="&idmp-uom;UnitOfPresentation"/>
		<rdfs:label>ampoule</rdfs:label>
		<skos:definition>presentation unit that is a sealed vial made of glass or plastic that contains a sterile medicinal solution or a powder that is usually made into a solution for subcutaneous, intramuscular, or intravenous injection</skos:definition>
	</owl:NamedIndividual>
	
	<owl:NamedIndividual rdf:about="&idmp-ucum;Dalton">
		<rdf:type rdf:resource="&cmns-qtu;ConversionBasedUnit"/>
		<rdfs:label>dalton</rdfs:label>
		<dct:source>https://ucum.org/ucum.html#section-Derived-Unit-Atoms</dct:source>
		<skos:definition>conversion-based unit of mass defined in the Unified Code for Units Of Measure (UCUM) System of Units</skos:definition>
		<idmp-uom:isSIQuantity rdf:datatype="&xsd;boolean">false</idmp-uom:isSIQuantity>
		<cmns-av:symbol>Da</cmns-av:symbol>
		<cmns-av:symbol>da</cmns-av:symbol>
		<cmns-dsg:hasDescription>1/12 of the mass of an unbound neutral atom of carbon-12 in its nuclear and electronic ground state and at rest, approximately 1.66×10^−27 kg</cmns-dsg:hasDescription>
		<cmns-dsg:isDefinedIn rdf:resource="&idmp-ucum;UnifiedCodeForUnitsOfMeasure"/>
		<cmns-qtu:hasQuantityKind rdf:resource="&idmp-ucum;Mass"/>
		<cmns-qtu:isDerivedFrom rdf:resource="&idmp-ucum;Kilogram"/>
	</owl:NamedIndividual>
	
	<owl:NamedIndividual rdf:about="&idmp-ucum;Dimension-L">
		<rdf:type rdf:resource="&cmns-qtu;QuantityDimension"/>
		<rdfs:label>dimension - L</rdfs:label>
		<skos:definition>dimension that is the measurement of how far apart objects or points are</skos:definition>
		<cmns-av:symbol>L</cmns-av:symbol>
		<cmns-cls:classifies rdf:resource="&idmp-ucum;Length"/>
		<cmns-dsg:isDefinedIn rdf:resource="&cmns-qtu;InternationalSystemOfQuantities"/>
	</owl:NamedIndividual>
	
	<owl:NamedIndividual rdf:about="&idmp-ucum;Dimension-M">
		<rdf:type rdf:resource="&cmns-qtu;QuantityDimension"/>
		<rdfs:label>dimension - M</rdfs:label>
		<skos:definition>dimension that is the measurement of a body&apos;s inertial property or how much matter it contains</skos:definition>
		<cmns-av:symbol>M</cmns-av:symbol>
		<cmns-cls:classifies rdf:resource="&idmp-ucum;Mass"/>
		<cmns-dsg:isDefinedIn rdf:resource="&cmns-qtu;InternationalSystemOfQuantities"/>
	</owl:NamedIndividual>
	
	<owl:NamedIndividual rdf:about="&idmp-ucum;Gram">
		<rdf:type rdf:resource="&cmns-qtu;BaseUnit"/>
		<rdfs:label>gram</rdfs:label>
		<dct:source>https://ucum.org/ucum.html#section-Base-Units</dct:source>
		<skos:definition>base unit of mass defined in the Unified Code for Units Of Measure (UCUM) System of Units</skos:definition>
		<idmp-uom:isSIQuantity rdf:datatype="&xsd;boolean">true</idmp-uom:isSIQuantity>
		<cmns-av:explanatoryNote>The kilogram, as of 2019, is defined by the International Bureau of Weights and Measures from the fixed numerical value of the Planck constant (h), which is 6.62607015×10^−34 kg⋅m^2⋅s^−1</cmns-av:explanatoryNote>
		<cmns-av:symbol>g</cmns-av:symbol>
		<cmns-dsg:isDefinedIn rdf:resource="&idmp-ucum;UnifiedCodeForUnitsOfMeasure"/>
	</owl:NamedIndividual>
	
	<owl:NamedIndividual rdf:about="&idmp-ucum;GramsPerMole">
		<rdf:type rdf:resource="&cmns-qtu;ConversionBasedUnit"/>
		<rdfs:label>grams per mole</rdfs:label>
		<dct:source>https://ucum.org/ucum.html#section-Derived-Unit-Atoms</dct:source>
		<skos:definition>conversion-based unit of molecular weight defined in the Unified Code for Units Of Measure (UCUM) System of Units</skos:definition>
		<idmp-uom:isSIQuantity rdf:datatype="&xsd;boolean">false</idmp-uom:isSIQuantity>
		<cmns-av:symbol>g/mol</cmns-av:symbol>
		<cmns-dsg:hasDescription>1.66054018667494 × 10^-21 kg</cmns-dsg:hasDescription>
		<cmns-dsg:isDefinedIn rdf:resource="&idmp-ucum;UnifiedCodeForUnitsOfMeasure"/>
		<cmns-qtu:hasQuantityKind rdf:resource="&idmp-ucum;MolarMass"/>
		<cmns-qtu:isDerivedFrom rdf:resource="&idmp-ucum;Gram"/>
		<cmns-qtu:isDerivedFrom rdf:resource="&idmp-ucum;Mole"/>
	</owl:NamedIndividual>
	
	<owl:NamedIndividual rdf:about="&idmp-ucum;Kilo">
		<rdf:type rdf:resource="&cmns-qtu;Prefix"/>
		<rdfs:label>kilo</rdfs:label>
		<dct:source>https://ucum.org/ucum.html#section-Prefixes</dct:source>
		<skos:definition>prefix defined in the Unified Code for Units Of Measure (UCUM) System of Units</skos:definition>
		<cmns-av:symbol>k</cmns-av:symbol>
		<cmns-dsg:hasDescription>10^3=(10^3)^1</cmns-dsg:hasDescription>
		<cmns-dsg:isDefinedIn rdf:resource="&idmp-ucum;UnifiedCodeForUnitsOfMeasure"/>
	</owl:NamedIndividual>
	
	<owl:NamedIndividual rdf:about="&idmp-ucum;Kilogram">
		<rdf:type rdf:resource="&cmns-qtu;PrefixedUnit"/>
		<rdfs:label>kilogram</rdfs:label>
		<dct:source>https://ucum.org/ucum.html#section-Base-Units</dct:source>
		<rdfs:seeAlso rdf:resource="https://www.nist.gov/si-redefinition/kilogram"/>
		<skos:definition>conversion-based unit of mass</skos:definition>
		<skos:note>Note that in the International System of Units (SI), the kilogram is considered the base unit rather than the gram, which is the base unit in the UCUM.</skos:note>
		<idmp-uom:isSIQuantity rdf:datatype="&xsd;boolean">true</idmp-uom:isSIQuantity>
		<cmns-av:symbol>kg</cmns-av:symbol>
		<cmns-dsg:hasDescription>10^3 grams</cmns-dsg:hasDescription>
		<cmns-dsg:isDefinedIn rdf:resource="&idmp-ucum;UnifiedCodeForUnitsOfMeasure"/>
		<cmns-dsg:isDefinedIn rdf:resource="&cmns-qtu;InternationalSystemOfUnits"/>
		<cmns-qtu:hasFactor rdf:resource="&idmp-ucum;Kilo"/>
		<cmns-qtu:hasQuantityKind rdf:resource="&idmp-ucum;Mass"/>
		<cmns-qtu:isDerivedFrom rdf:resource="&idmp-ucum;Gram"/>
	</owl:NamedIndividual>
	
	<owl:NamedIndividual rdf:about="&idmp-ucum;Length">
		<rdf:type rdf:resource="&cmns-qtu;BaseQuantityKind"/>
		<rdfs:label>length</rdfs:label>
		<dct:source>https://ucum.org/ucum.html#section-Base-Units</dct:source>
		<skos:definition>base quantity kind that is the quantitative measure of distance, i.e., of how far apart objects or points are</skos:definition>
		<cmns-av:symbol>l</cmns-av:symbol>
		<cmns-dsg:isDefinedIn rdf:resource="&idmp-ucum;UnifiedCodeForUnitsOfMeasure"/>
		<cmns-dsg:isDefinedIn rdf:resource="&cmns-qtu;InternationalSystemOfQuantities"/>
		<cmns-qtu:hasDimension rdf:resource="&idmp-ucum;Dimension-L"/>
	</owl:NamedIndividual>
	
	<owl:NamedIndividual rdf:about="&idmp-ucum;Liter">
		<rdf:type rdf:resource="&cmns-qtu;ConversionBasedUnit"/>
		<rdfs:label>liter</rdfs:label>
		<dct:source>https://ucum.org/ucum.html#section-Derived-Unit-Atoms</dct:source>
		<skos:definition>derived unit of volume defined in the Unified Code for Units Of Measure (UCUM) System of Units</skos:definition>
		<idmp-uom:isSIQuantity rdf:datatype="&xsd;boolean">true</idmp-uom:isSIQuantity>
		<cmns-av:symbol>l</cmns-av:symbol>
		<cmns-dsg:hasDescription>cubic meter: m^3</cmns-dsg:hasDescription>
		<cmns-dsg:isDefinedIn rdf:resource="&idmp-ucum;UnifiedCodeForUnitsOfMeasure"/>
		<cmns-qtu:hasQuantityKind rdf:resource="&idmp-ucum;Volume"/>
		<cmns-qtu:isDerivedFrom rdf:resource="&idmp-ucum;Meter"/>
	</owl:NamedIndividual>
	
	<owl:NamedIndividual rdf:about="&idmp-ucum;Mass">
		<rdf:type rdf:resource="&cmns-qtu;BaseQuantityKind"/>
		<rdfs:label>mass</rdfs:label>
		<skos:definition>base quantity kind for the measure of a measure of a body&apos;s inertial property or how much matter it contains</skos:definition>
		<cmns-av:explanatoryNote>Note that as of 2018, mass has been redefined in the International System of Units in terms of Planck&apos;s constant, h. The kilogram is defined by taking the fixed numerical value of the Planck constant, h, to be 6.626 070 15 × 10-34 when expressed in the unit J s, which is equal to kg m^2 s^−1, where the metre and the second are defined in terms of the speed of light, 𝒸, and the hyperfine transition frequency of the caesium-133 atom, ∆ν, respectively.</cmns-av:explanatoryNote>
		<cmns-av:symbol>m</cmns-av:symbol>
		<cmns-dsg:isDefinedIn rdf:resource="&idmp-ucum;UnifiedCodeForUnitsOfMeasure"/>
		<cmns-qtu:hasDimension rdf:resource="&idmp-ucum;Dimension-M"/>
	</owl:NamedIndividual>
	
	<owl:NamedIndividual rdf:about="&idmp-ucum;MassConcentration">
		<rdf:type rdf:resource="&cmns-qtu;DerivedQuantityKind"/>
		<rdfs:label>mass concentration</rdfs:label>
		<dct:source>ISO 31-0:1992(E) Quantities and Units - Part 0: General principles, clause A.6.6</dct:source>
		<dct:source>https://ucum.org/ucum.html#section-Base-Units</dct:source>
		<skos:definition>derived quantity kind defined in the International System of Quantities for the quantitative measure of the mass of a constituent divided by the total volume of the mixture</skos:definition>
		<cmns-av:explanatoryNote>For a pure chemical the mass concentration equals its density (mass divided by volume); thus the mass concentration of a component in a mixture can be called the density of a component in a mixture.</cmns-av:explanatoryNote>
		<cmns-av:explanatoryNote>Note that the Unified Code for Units Of Measure (UCUM) uses mass concentration primarily with respect to gram percent, which is a dimensionless unit in that system.</cmns-av:explanatoryNote>
		<cmns-av:symbol>ML^3</cmns-av:symbol>
		<cmns-av:symbol>γ</cmns-av:symbol>
		<cmns-av:symbol>ρ</cmns-av:symbol>
		<cmns-dsg:isDefinedIn rdf:resource="&cmns-qtu;InternationalSystemOfQuantities"/>
		<cmns-qtu:isDerivedFrom rdf:resource="&idmp-ucum;Mass"/>
	</owl:NamedIndividual>
	
	<owl:NamedIndividual rdf:about="&idmp-ucum;Meter">
		<rdf:type rdf:resource="&cmns-qtu;BaseUnit"/>
		<rdfs:label>meter</rdfs:label>
		<dct:source>https://ucum.org/ucum.html#section-Base-Units</dct:source>
		<rdfs:seeAlso rdf:resource="https://www.nist.gov/pml/owm/si-units-length"/>
		<rdfs:seeAlso rdf:resource="https://www.nist.gov/system/files/documents/pml/div683/museum-length.pdf"/>
		<skos:definition>base unit of length that is the distance traveled by light in vacuum during the time interval of 1/299 792 458 of a second</skos:definition>
		<idmp-uom:isSIQuantity rdf:datatype="&xsd;boolean">true</idmp-uom:isSIQuantity>
		<cmns-av:symbol>m</cmns-av:symbol>
		<cmns-dsg:isDefinedIn rdf:resource="&idmp-ucum;UnifiedCodeForUnitsOfMeasure"/>
		<cmns-dsg:isDefinedIn rdf:resource="&cmns-qtu;InternationalSystemOfUnits"/>
	</owl:NamedIndividual>
	
	<owl:NamedIndividual rdf:about="&idmp-ucum;Micro">
		<rdf:type rdf:resource="&cmns-qtu;Prefix"/>
		<rdfs:label>micro</rdfs:label>
		<dct:source>https://ucum.org/ucum.html#section-Prefixes</dct:source>
		<skos:definition>prefix defined in the Unified Code for Units Of Measure (UCUM) System of Units</skos:definition>
		<cmns-av:symbol>μ</cmns-av:symbol>
		<cmns-dsg:hasDescription>10^-6=(10^3)^-2</cmns-dsg:hasDescription>
		<cmns-dsg:isDefinedIn rdf:resource="&idmp-ucum;UnifiedCodeForUnitsOfMeasure"/>
	</owl:NamedIndividual>
	
	<owl:NamedIndividual rdf:about="&idmp-ucum;Microgram">
		<rdf:type rdf:resource="&cmns-qtu;PrefixedUnit"/>
		<rdfs:label>microgram</rdfs:label>
		<dct:source>https://ucum.org/ucum.html#section-Derived-Unit-Atoms</dct:source>
		<skos:definition>conversion-based unit of mass defined in the Unified Code for Units Of Measure (UCUM) System of Units</skos:definition>
		<idmp-uom:isSIQuantity rdf:datatype="&xsd;boolean">true</idmp-uom:isSIQuantity>
		<cmns-av:symbol>mcg</cmns-av:symbol>
		<cmns-av:symbol>μg</cmns-av:symbol>
		<cmns-dsg:hasDescription>10^-6 grams</cmns-dsg:hasDescription>
		<cmns-dsg:isDefinedIn rdf:resource="&idmp-ucum;UnifiedCodeForUnitsOfMeasure"/>
		<cmns-qtu:hasFactor rdf:resource="&idmp-ucum;Micro"/>
		<cmns-qtu:hasQuantityKind rdf:resource="&idmp-ucum;Mass"/>
		<cmns-qtu:isDerivedFrom rdf:resource="&idmp-ucum;Gram"/>
	</owl:NamedIndividual>
	
	<owl:NamedIndividual rdf:about="&idmp-ucum;MicrogramsPerMilliliter">
		<rdf:type rdf:resource="&cmns-qtu;PrefixedUnit"/>
		<rdfs:label>micrograms per milliliter</rdfs:label>
		<dct:source>https://ucum.org/ucum.html#section-Derived-Unit-Atoms</dct:source>
		<skos:definition>conversion-based unit of mass concentration (density) used to measure volume in milliliters in order to estimate weight or mass in micrograms</skos:definition>
		<idmp-uom:isSIQuantity rdf:datatype="&xsd;boolean">true</idmp-uom:isSIQuantity>
		<cmns-av:symbol>μg/ml</cmns-av:symbol>
		<cmns-dsg:hasDescription>10^-6 grams per 10^-3 liters</cmns-dsg:hasDescription>
		<cmns-dsg:isDefinedIn rdf:resource="&idmp-ucum;UnifiedCodeForUnitsOfMeasure"/>
		<cmns-qtu:hasFactor rdf:resource="&idmp-ucum;Micro"/>
		<cmns-qtu:hasQuantityKind rdf:resource="&idmp-ucum;MassConcentration"/>
		<cmns-qtu:isDerivedFrom rdf:resource="&idmp-ucum;Gram"/>
		<cmns-qtu:isDerivedFrom rdf:resource="&idmp-ucum;Liter"/>
	</owl:NamedIndividual>
	
	<owl:NamedIndividual rdf:about="&idmp-ucum;Milli">
		<rdf:type rdf:resource="&cmns-qtu;Prefix"/>
		<rdfs:label>milli</rdfs:label>
		<dct:source>https://ucum.org/ucum.html#section-Prefixes</dct:source>
		<skos:definition>prefix defined in the Unified Code for Units Of Measure (UCUM) System of Units</skos:definition>
		<cmns-av:symbol>m</cmns-av:symbol>
		<cmns-dsg:hasDescription>10^-3=(10^3)-1</cmns-dsg:hasDescription>
		<cmns-dsg:isDefinedIn rdf:resource="&idmp-ucum;UnifiedCodeForUnitsOfMeasure"/>
	</owl:NamedIndividual>
	
	<owl:NamedIndividual rdf:about="&idmp-ucum;Milligram">
		<rdf:type rdf:resource="&cmns-qtu;PrefixedUnit"/>
		<rdfs:label>milligram</rdfs:label>
		<dct:source>https://ucum.org/ucum.html#section-Derived-Unit-Atoms</dct:source>
		<skos:definition>conversion-based unit of mass defined in the Unified Code for Units Of Measure (UCUM) System of Units</skos:definition>
		<idmp-uom:isSIQuantity rdf:datatype="&xsd;boolean">true</idmp-uom:isSIQuantity>
		<cmns-av:symbol>mg</cmns-av:symbol>
		<cmns-dsg:hasDescription>10^-3 grams</cmns-dsg:hasDescription>
		<cmns-dsg:isDefinedIn rdf:resource="&idmp-ucum;UnifiedCodeForUnitsOfMeasure"/>
		<cmns-qtu:hasFactor rdf:resource="&idmp-ucum;Milli"/>
		<cmns-qtu:hasQuantityKind rdf:resource="&idmp-ucum;Mass"/>
		<cmns-qtu:isDerivedFrom rdf:resource="&idmp-ucum;Gram"/>
	</owl:NamedIndividual>
	
	<owl:NamedIndividual rdf:about="&idmp-ucum;MilligramsPerMilliliter">
		<rdf:type rdf:resource="&cmns-qtu;PrefixedUnit"/>
		<rdfs:label>milligrams per milliliter</rdfs:label>
		<dct:source>https://ucum.org/ucum.html#section-Derived-Unit-Atoms</dct:source>
		<skos:definition>conversion-based unit of mass concentration (density) used to measure volume in milliliters in order to estimate weight or mass in milligrams</skos:definition>
		<idmp-uom:isSIQuantity rdf:datatype="&xsd;boolean">true</idmp-uom:isSIQuantity>
		<cmns-av:symbol>mg/ml</cmns-av:symbol>
		<cmns-dsg:hasDescription>10^-3 grams per 10^-3 liters</cmns-dsg:hasDescription>
		<cmns-dsg:isDefinedIn rdf:resource="&idmp-ucum;UnifiedCodeForUnitsOfMeasure"/>
		<cmns-qtu:hasFactor rdf:resource="&idmp-ucum;Milli"/>
		<cmns-qtu:hasQuantityKind rdf:resource="&idmp-ucum;MassConcentration"/>
		<cmns-qtu:isDerivedFrom rdf:resource="&idmp-ucum;Gram"/>
		<cmns-qtu:isDerivedFrom rdf:resource="&idmp-ucum;Liter"/>
	</owl:NamedIndividual>
	
	<owl:NamedIndividual rdf:about="&idmp-ucum;Milliliter">
		<rdf:type rdf:resource="&cmns-qtu;PrefixedUnit"/>
		<rdfs:label>milliliter</rdfs:label>
		<dct:source>https://ucum.org/ucum.html#section-Derived-Unit-Atoms</dct:source>
		<skos:definition>conversion-based unit of volume defined in the Unified Code for Units Of Measure (UCUM) System of Units</skos:definition>
		<idmp-uom:isSIQuantity rdf:datatype="&xsd;boolean">true</idmp-uom:isSIQuantity>
		<cmns-av:symbol>ml</cmns-av:symbol>
		<cmns-dsg:hasDescription>10^-3 liters</cmns-dsg:hasDescription>
		<cmns-dsg:isDefinedIn rdf:resource="&idmp-ucum;UnifiedCodeForUnitsOfMeasure"/>
		<cmns-qtu:hasFactor rdf:resource="&idmp-ucum;Milli"/>
		<cmns-qtu:hasQuantityKind rdf:resource="&idmp-ucum;Volume"/>
		<cmns-qtu:isDerivedFrom rdf:resource="&idmp-ucum;Liter"/>
	</owl:NamedIndividual>
	
	<owl:NamedIndividual rdf:about="&idmp-ucum;MolarMass">
		<rdf:type rdf:resource="&cmns-qtu;DerivedQuantityKind"/>
		<rdfs:label>molar mass</rdfs:label>
		<dct:source>https://ucum.org/ucum.html#section-Derived-Unit-Atoms</dct:source>
		<skos:definition>derived quantity kind defined in the Unified Code for Units Of Measure (UCUM) System of Units for the mass of a substance divided by its amount of substance in moles</skos:definition>
		<skos:example>For example, the molar mass of water (H2O) is approximately 1 × 2 + 16 = 18 g/mol.</skos:example>
		<skos:note>The molar mass of elements in grams per mole is numerically equal to their atomic mass in unified atomic mass units (u) or daltons (Da). The molar mass of compounds is equal to the sum of molar masses of the atoms which form the compound.</skos:note>
		<cmns-dsg:isDefinedIn rdf:resource="&idmp-ucum;UnifiedCodeForUnitsOfMeasure"/>
		<cmns-qtu:isDerivedFrom rdf:resource="&idmp-ucum;Mass"/>
	</owl:NamedIndividual>
	
	<owl:NamedIndividual rdf:about="&idmp-ucum;Mole">
		<rdf:type rdf:resource="&cmns-qtu;BaseUnit"/>
		<rdfs:label>mole</rdfs:label>
		<dct:source>https://ucum.org/ucum.html#section-Base-Units</dct:source>
		<rdfs:seeAlso rdf:resource="https://www.nist.gov/system/files/documents/pml/div683/museum-length.pdf"/>
		<skos:definition>base unit of amount of substance defined in the Unified Code for Units Of Measure (UCUM) System of Units that is the measure of how many elementary entities of a given substance are in an object or sample</skos:definition>
		<idmp-uom:isSIQuantity rdf:datatype="&xsd;boolean">true</idmp-uom:isSIQuantity>
		<cmns-av:symbol>mol</cmns-av:symbol>
		<cmns-dsg:hasDescription>6.02214076×10^23 elementary entities</cmns-dsg:hasDescription>
		<cmns-dsg:isDefinedIn rdf:resource="&idmp-ucum;UnifiedCodeForUnitsOfMeasure"/>
	</owl:NamedIndividual>
	
	<owl:NamedIndividual rdf:about="&idmp-ucum;OID-2.16.840.1.113883.6.8">
		<rdf:type rdf:resource="&idmp-uom;CodeSystemIdentifier"/>
		<rdfs:label>Unified Code for Units of Measure identifier</rdfs:label>
		<dct:source>ISO 11240:2021, clause 4.6.2.2 and clause 4.6.2.3 Code System, Table 3</dct:source>
		<skos:definition>ISO Object Identifier (OID) for the Unified Code for Units of Measure (UCUM) code set</skos:definition>
		<idmp-dtp:isEncodedAs rdf:resource="&idmp-dtp;DatatypeCode-ST"/>
		<cmns-id:identifies rdf:resource="&idmp-ucum;UnifiedCodeForUnitsOfMeasure"/>
		<cmns-txt:hasTextValue>2.16.840.1.113883.6.8</cmns-txt:hasTextValue>
	</owl:NamedIndividual>
	
	<owl:NamedIndividual rdf:about="&idmp-ucum;Tablet">
		<rdf:type rdf:resource="&idmp-uom;UnitOfPresentation"/>
		<rdfs:label>tablet</rdfs:label>
		<skos:definition>presentation unit that is a solid unit dosage form of one or more medicaments with or without suitable excipients and prepared either by molding or by compression</skos:definition>
	</owl:NamedIndividual>
	
	<owl:NamedIndividual rdf:about="&idmp-ucum;UnifiedAtomicMassUnit">
		<rdf:type rdf:resource="&cmns-qtu;ConversionBasedUnit"/>
		<rdfs:label>unified atomic mass unit</rdfs:label>
		<dct:source>https://ucum.org/ucum.html#section-Derived-Unit-Atoms</dct:source>
		<skos:definition>conversion-based unit of mass defined in the Unified Code for Units Of Measure (UCUM) System of Units</skos:definition>
		<idmp-uom:isSIQuantity rdf:datatype="&xsd;boolean">true</idmp-uom:isSIQuantity>
		<cmns-av:symbol>AMU</cmns-av:symbol>
		<cmns-av:symbol>u</cmns-av:symbol>
		<cmns-dsg:hasDescription>1.6605402 × 10^-24 kg</cmns-dsg:hasDescription>
		<cmns-dsg:isDefinedIn rdf:resource="&idmp-ucum;UnifiedCodeForUnitsOfMeasure"/>
		<cmns-qtu:hasQuantityKind rdf:resource="&idmp-ucum;Mass"/>
		<cmns-qtu:isDerivedFrom rdf:resource="&idmp-ucum;Kilogram"/>
	</owl:NamedIndividual>
	
	<owl:NamedIndividual rdf:about="&idmp-ucum;UnifiedCodeForUnitsOfMeasure">
		<rdf:type rdf:resource="&idmp-uom;UnitOfMeasureIdentificationScheme"/>
		<rdfs:label>Unified Code for Units of Measure</rdfs:label>
		<rdfs:seeAlso rdf:resource="https://ucum.nlm.nih.gov/"/>
		<rdfs:seeAlso rdf:resource="https://ucum.org/trac"/>
		<owl:versionInfo>Version: 2.1, Revision: 442</owl:versionInfo>
		<skos:definition>code system intended to include all units of measures being contemporarily used in international science, engineering, and business</skos:definition>
		<skos:note>UCUM has been adopted internationally by many organizations such as IEEE, DICOM, LOINC, and HL7, and is also in the ISO 11240:2012 standard</skos:note>
		<cmns-av:abbreviation>UCUM</cmns-av:abbreviation>
		<cmns-av:copyright>Copyright 1999-2021 Regenstrief Institute, Inc. All rights reserved.</cmns-av:copyright>
		<cmns-dsg:hasDescription>The Unified Code for Units of Measure (UCUM) was developed by Regenstrief Institute and the UCUM Organization as a unambiguous system of units and their combinations. The purpose is to facilitate unambiguous electronic communication of quantities together with their units. The focus is on electronic communication, as opposed to communication between humans. A typical application of The Unified Code for Units of Measure are electronic data interchange (EDI) protocols, but there is nothing that prevents it from being used in other types of machine communication.</cmns-dsg:hasDescription>
		<cmns-dsg:hasName rdf:resource="&idmp-ucum;UnifiedCodeForUnitsOfMeasureCodeSystemFullName"/>
		<cmns-dsg:hasName rdf:resource="&idmp-ucum;UnifiedCodeForUnitsOfMeasureCodeSystemName"/>
		<cmns-id:isIdentifiedBy rdf:resource="&idmp-ucum;OID-2.16.840.1.113883.6.8"/>
	</owl:NamedIndividual>
	
	<owl:NamedIndividual rdf:about="&idmp-ucum;UnifiedCodeForUnitsOfMeasureCodeSystemFullName">
		<rdf:type rdf:resource="&idmp-uom;CodeSystemFullName"/>
		<rdfs:label>Unified Code for Units of Measure code system full name</rdfs:label>
		<dct:source>ISO 11240:2021, clause 4.6.2.3 Code System, Table 3</dct:source>
		<skos:definition>official name for the Unified Code for Units of Measure code system</skos:definition>
		<idmp-dtp:isEncodedAs rdf:resource="&idmp-dtp;DatatypeCode-ST"/>
		<cmns-dsg:isNameOf rdf:resource="&idmp-ucum;UnifiedCodeForUnitsOfMeasure"/>
		<cmns-txt:hasTextValue>Unified Code for Units of Measure</cmns-txt:hasTextValue>
	</owl:NamedIndividual>
	
	<owl:NamedIndividual rdf:about="&idmp-ucum;UnifiedCodeForUnitsOfMeasureCodeSystemName">
		<rdf:type rdf:resource="&idmp-dtp;CodeSystemName"/>
		<rdfs:label>Unified Code for Units of Measure code system name</rdfs:label>
		<dct:source>ISO 11240:2021, clause 4.6.2.3 Code System, Table 3</dct:source>
		<skos:definition>short name that uniquely identifies the Unified Code for Units of Measure code system for communications between people</skos:definition>
		<idmp-dtp:isEncodedAs rdf:resource="&idmp-dtp;DatatypeCode-ST"/>
		<cmns-dsg:isNameOf rdf:resource="&idmp-ucum;UnifiedCodeForUnitsOfMeasure"/>
		<cmns-txt:hasTextValue>UCUM</cmns-txt:hasTextValue>
	</owl:NamedIndividual>
	
	<owl:NamedIndividual rdf:about="&idmp-ucum;Volume">
		<rdf:type rdf:resource="&cmns-qtu;DerivedQuantityKind"/>
		<rdfs:label>volume</rdfs:label>
		<dct:source>https://ucum.org/ucum.html#section-Derived-Unit-Atoms</dct:source>
		<skos:definition>derived quantity kind defined in the Unified Code for Units Of Measure (UCUM) System of Units for the quantitative measure expressing the amount of three-dimensional space enclosed by a closed surface</skos:definition>
		<cmns-av:symbol>L^3</cmns-av:symbol>
		<cmns-dsg:isDefinedIn rdf:resource="&idmp-ucum;UnifiedCodeForUnitsOfMeasure"/>
		<cmns-qtu:isDerivedFrom rdf:resource="&idmp-ucum;Length"/>
	</owl:NamedIndividual>
	
	<owl:Class rdf:about="&idmp-uom;ISO11240LexiconCodeEntry">
		<rdfs:subClassOf>
			<owl:Restriction>
				<owl:onProperty rdf:resource="&cmns-col;compliesWith"/>
				<owl:hasValue rdf:resource="&idmp-ucum;UnifiedCodeForUnitsOfMeasure"/>
			</owl:Restriction>
		</rdfs:subClassOf>
		<rdfs:subClassOf>
			<owl:Restriction>
				<owl:onProperty rdf:resource="&cmns-col;isMemberOf"/>
				<owl:hasValue rdf:resource="&idmp-ucum;UnifiedCodeForUnitsOfMeasure"/>
			</owl:Restriction>
		</rdfs:subClassOf>
	</owl:Class>

</rdf:RDF>